Alg/Nat/PrimeFactors/Intersect.lean
@@ -1,76 +1,124 @@
 import Alg.Nat.PrimeFactors
 import Alg.ListProps.Sorted.Intersect
 
+def contrapositive : (P -> Q) -> ¬ Q -> ¬ P := by
+  intro p_to_q not_q p
+  exact not_q (p_to_q p)
+
 theorem list_product.of_sorted_intersect :
   ∀{as bs: List nat},
-  list_product (as.sorted_intersect bs) = (list_product as) * (list_product bs) := by
+  as.sorted ->
+  bs.sorted ->
+  as.allP nat.prime ->
+  bs.allP nat.prime ->
+  list_product (as.sorted_intersect bs) = (list_product as).gcd (list_product bs) := by
   apply List.sorted.induction
   {
     intro bs
-    rw [List.sorted_intersect.empty_left, list_product.empty, nat.mul_one_left]
+    intro _ _ _ _
+    rw [List.sorted_intersect.empty_left, list_product.empty]
+    rw [nat.gcd.one_left]
   }
   {
     intro a as
-    rw [List.sorted_intersect.empty_right, list_product.empty, nat.mul_one_right]
+    intro _ _ _ _
+    rw [List.sorted_intersect.empty_right, list_product.empty]
+    rw [nat.gcd.one_right]
   }
   {
     intro a as b bs a_ord_b prev
+    intro as_sort bs_sort as_primes bs_primes
     rw [List.sorted_intersect.induct_lt a_ord_b]
     conv => {
-      lhs
-      unfold list_product
-    }
-    conv => {
       rhs
       lhs
       unfold list_product
     }
-    rw [nat.mul_perm_ab_c_to_a_bc]
-    apply nat.to_mul_irr_left
-    assumption
+
+    rw [nat.gcd.cancel_left]
+    {
+      apply prev
+      exact as_sort.pop
+      assumption
+      exact as_primes.right
+      assumption
+    }
+    {
+      have not_con := List.not_contains_sorted a_ord_b bs_sort
+      generalize b_fact_def:PrimeFactorization.mk (b::bs) bs_primes rfl bs_sort = b_fact
+      have b_complete := b_fact.is_complete a as_primes.left
+      rw [←b_fact_def] at b_complete
+      have not_dvd := contrapositive b_complete not_con
+      match nat.prime.to_coprime_or_dvd as_primes.left (list_product (b::bs)) with
+      | .inr _ => contradiction
+      | .inl a_coprime_bs => exact a_coprime_bs
+    }
   }
   {
     intro a as b bs a_ord_b prev
+    intro as_sort bs_sort as_primes bs_primes
     rw [List.sorted_intersect.induct_eq a_ord_b]
     simp
-    rw [nat.mul_perm_ab_c_to_a_bc]
+    have a_eq_b : a = b := Compare.ord_to_eq a_ord_b
+    rw [←a_eq_b, nat.gcd.mul_left]
     apply nat.to_mul_irr_left
-    rw [nat.mul_perm_a_bc_to_b_ac]
-    apply nat.to_mul_irr_left
-    assumption
+    apply prev
+    exact as_sort.pop
+    exact bs_sort.pop
+    exact as_primes.right
+    exact bs_primes.right
   }
   {
     intro a as b bs a_ord_b prev
+    intro as_sort bs_sort as_primes bs_primes
     rw [List.sorted_intersect.induct_gt a_ord_b]
     conv => {
-      lhs
-      unfold list_product
-    }
-    conv => {
       rhs
       rhs
       unfold list_product
     }
-    rw [nat.mul_perm_a_bc_to_b_ac]
-    apply nat.to_mul_irr_left
-    assumption
+
+    rw [nat.gcd.comm, nat.gcd.cancel_left, nat.gcd.comm]
+    {
+      apply prev
+      assumption
+      exact bs_sort.pop
+      assumption
+      exact bs_primes.right
+    }
+    {
+      have not_con := List.not_contains_sorted (Compare.flip a_ord_b) as_sort
+      generalize a_fact_def:PrimeFactorization.mk (a::as) as_primes rfl as_sort = a_fact
+      have a_complete := a_fact.is_complete b bs_primes.left
+      rw [←a_fact_def] at a_complete
+      have not_dvd := contrapositive a_complete not_con
+      match nat.prime.to_coprime_or_dvd bs_primes.left (list_product (a::as)) with
+      | .inr _ => contradiction
+      | .inl a_coprime_bs => exact a_coprime_bs
+    }
   }
 
 #print axioms list_product.of_sorted_intersect
 
-theorem PrimeFactorization.merge
+theorem PrimeFactorization.intersect
   (fa: PrimeFactorization a)
   (fb: PrimeFactorization b):
   PrimeFactorization (a.gcd b) := by
   apply PrimeFactorization.mk (fa.factors.sorted_intersect fb.factors)
-  apply List.sorted_intersect.keeps_allP
+  apply List.sublist_of.allP
+  apply List.sorted_intersect.sublist_of_left
+  exact fa.sorted
+  exact fb.sorted
   exact fa.all_primes
-  exact fb.all_primes
   rw [list_product.of_sorted_intersect]
   rw [←fa.eq_n]
   rw [←fb.eq_n]
+  exact fa.sorted
+  exact fb.sorted
+  exact fa.all_primes
+  exact fb.all_primes
   apply List.sorted_intersect.keeps_sorted
   exact fa.sorted
   exact fb.sorted
 
-#print axioms PrimeFactorization.merge
+#print axioms PrimeFactorization.intersect
